1. I)

> $$V = \pi \int_{a}^{b} [f(x)]^2 \, dx$$
   $$
   f(x)^2 = (2x^4 + 1)^2 = 4x^8 + 4x^4 + 1
   $$
$$
V = \pi \int_{0}^{1} (4x^8 + 4x^4 + 1) \, dx
$$
$$( 4x^8 ) = ( \frac{4}{9} x^9 )$$
$$( 4x^4 ) = ( \frac{4}{5} x^5 )$$
$$( 1 ) = ( x )$$
$$
V = \pi \left[ \frac{4}{9} x^9 + \frac{4}{5} x^5 + x \right]_{0}^{1} 
$$
$$
= \pi \left( \frac{4}{9} (1)^9 + \frac{4}{5} (1)^5 + (1) \right) - \pi \left( \frac{4}{9} (0)^9 + \frac{4}{5} (0)^5 + (0) \right) = \pi \left( \frac{4}{9} + \frac{4}{5} + 1 \right) 
$$
$$
\frac{4}{9} = \frac{20}{45} ;
\frac{4}{5} = \frac{36}{45} ;
1 = \frac{45}{45} 
$$
   $$
   \frac{20}{45} + \frac{36}{45} + \frac{45}{45} = \frac{101}{45}
   $$
$$
V = \pi \left( \frac{101}{45} \right) = \frac{101\pi}{45}
$$
2. 


> $$A = \int_{1}^{2} \sqrt{2x} \, dx$$

$$
A = \int_{1}^{2} (2x)^{1/2} \, dx$$
$$ = \int_{1}^{2} 2^{1/2} x^{1/2} \, dx $$
$$ = \sqrt{2} \int_{1}^{2} x^{1/2} \, dx $$
$$ = \sqrt{2} \left[ \frac{2}{3} x^{3/2} \right]_{1}^{2} $$
$$ = \sqrt{2} \left( \frac{2}{3} (2^{3/2}) - \frac{2}{3} (1^{3/2}) \right) $$
$$ = \sqrt{2} \left( \frac{2}{3} (2\sqrt{2}) - \frac{2}{3} (1) \right) $$
$$= \sqrt{2} \left( \frac{4}{3} - \frac{2}{3} \right)$$
$$= \sqrt{2} \cdot \frac{2}{3} = \frac{2\sqrt{2}}{3}$$
$$
\bar{x} = \frac{1}{A} \int_{1}^{2} x \cdot \sqrt{2x} dx 
$$
$$
= \frac{1}{\frac{2\sqrt{2}}{3}} \int_{1}^{2} x \sqrt{2x} \, dx 
$$
$$ = \frac{3}{2\sqrt{2}} \int_{1}^{2} \sqrt{2} x^{3/2} \, dx $$
$$ 
= \frac{3}{2\sqrt{2}} \cdot \sqrt{2} \int_{1}^{2} x^{3/2} \, dx
$$
$$ 
= \frac{3}{2} \left[ \frac{2}{5} x^{5/2} \right]_{1}^{2} 
$$
$$ 
= \frac{3}{2} \cdot \frac{2}{5} \left(  (2^{5/2}) - (1^{5/2}) \right)
$$
$$
= \frac{3}{5} \left( 4\sqrt{2} - 1 \right)
$$
$$
\bar{y} = \frac{1}{A} \int_{1}^{2} \frac{1}{2} (\sqrt{2x})^2 \, dx 
$$
$$
= \frac{1}{\frac{2\sqrt{2}}{3}} \int_{1}^{2} \frac{1}{2} (2x) \, dx 
$$
$$
= \frac{3}{2\sqrt{2}} \cdot \int_{1}^{2} x \, dx 
$$
$$
= \frac{3}{2\sqrt{2}} \left[ \frac{1}{2} x^2 \right]_{1}^{2} 
$$
$$
= \frac{3}{2\sqrt{2}} \cdot \frac{1}{2} \left( 2^2 - 1^2 \right) 
$$
$$
= \frac{3}{2\sqrt{2}} \cdot \frac{1}{2} (4 - 1) 
$$
$$
= \frac{3}{2\sqrt{2}} \cdot \frac{3}{2} = \frac{9}{4\sqrt{2}} = \frac{9\sqrt{2}}{8}
$$
$$
\bar{x} = \frac{3}{5} (4\sqrt{2} - 1), \quad \bar{y} = \frac{9\sqrt{2}}{8}
$$
